pop2022: soundness proof and bank account & examples in paper

coq_inference/classical.v
@@ -4,7 +4,9 @@ Require Import partial_maps.
 Require Import L_def.
 Require Import exp.
 Require Import exp_properties.
+Require Import operational_semantics.
 Require Import chainmail.
+Require Import chainmail_tactics.
 Require Import List.
 Require Import String.
 Open Scope string_scope.
@@ -14,21 +16,20 @@ Require Import Coq.Logic.FunctionalExtensionality.
 Module ClassicalProperties(L : LanguageDef).
 
   Import L.
-  Module L_Chainmail := Chainmail(L).
-  Import L_Chainmail.
-  Import L_Semantics.
+  Module L_ChainmailTactics := ChainmailTactics(L).
+  Export L_ChainmailTactics.
   Open Scope reduce_scope.
   Open Scope chainmail_scope.
 
   Ltac sat_contra_inversion :=
     match goal with
-    | [|- ~ _ ⦂ _ ◎ _ … _ ⊨ _] =>
+    | [|- ~ _ ⦂ _ ◎ _ ⊨ _] =>
       let Hcontra := fresh in
       intro Hcontra;
       inversion Hcontra;
       subst;
       clear Hcontra
-    | [|- ~ _ ⦂ _ ◎ _ … _ ⊭ _] =>
+    | [|- ~ _ ⦂ _ ◎ _ ⊭ _] =>
       let Hcontra := fresh in
       intro Hcontra;
       inversion Hcontra;
@@ -39,85 +40,13 @@ Module ClassicalProperties(L : LanguageDef).
       intro Hcontra
     end.
 
-
-Lemma restrict_unique :
-  forall Σ χ χ1 χ2, restrict Σ χ χ1 ->
-               restrict Σ χ χ2 ->
-               χ1 = χ2.
-Proof.
-  intros;
-    repeat match goal with
-           | [H : restrict _ _ _ |- _ ] =>
-             inversion H;
-               subst;
-               clear H
-           end.
-  apply functional_extensionality;
-    intros.
-  destruct (partial_map_dec x χ1) as [Hsome1 | Hnone1];
-    destruct (partial_map_dec x χ2) as [Hsome2 | Hnone2];
-    repeat destruct_exists_loo;
-    try rewrite Hsome1;
-    try rewrite Hsome2;
-    try rewrite Hnone1;
-    try rewrite Hnone2;
-    auto.
-
-  - repeat match goal with
-           | [Ha : forall y o', ?m y = Some o' -> _ ,
-                Hb : ?m ?x = Some ?o |- context [?m ?x]] =>
-             specialize (Ha x o);
-               auto_specialize
-           end.
-    repeat simpl_crush;
-      crush.
-
-  - repeat match goal with
-           | [Ha : forall y o', ?m y = Some o' -> _ ,
-                Hb : ?m ?x = Some ?o |- context [?m ?x]] =>
-             specialize (Ha x o);
-               auto_specialize
-           end.
-    repeat match goal with
-           | [Ha : forall y, set_In (a_ y) ?Σ -> _ ,
-                Hb : set_In (a_ ?x) ?Σ |- _ ] =>
-             specialize (Ha x);
-               auto_specialize
-           end;
-      repeat destruct_exists_loo;
-      repeat simpl_crush.
-
-  -  repeat match goal with
-           | [Ha : forall y o', ?m y = Some o' -> _ ,
-                Hb : ?m ?x = Some ?o |- context [?m ?x]] =>
-             specialize (Ha x o);
-               auto_specialize
-           end.
-    repeat match goal with
-           | [Ha : forall y, set_In (a_ y) ?Σ -> _ ,
-                Hb : set_In (a_ ?x) ?Σ |- _ ] =>
-             specialize (Ha x);
-               auto_specialize
-           end;
-      repeat destruct_exists_loo;
-      repeat simpl_crush.
-Qed.
-
-Ltac unique_restriction :=
-  match goal with
-  | [Ha : restrict ?Σ ?χ ?χ1,
-          Hb : restrict ?Σ ?χ ?χ2 |- _ ] =>
-    assert (χ1 = χ2);
-    [eapply restrict_unique; eauto|subst; clear Hb]
-  end.
-
   (** Lemma 5: Classical (4) *)
   Theorem sat_implies_not_nsat_mutind :
-    (forall M1 M2 σ0 σ A, M1 ⦂ M2 ◎ σ0 … σ ⊨ A ->
-                     ~ M1 ⦂ M2 ◎ σ0 … σ ⊭ A) /\
+    (forall M1 M2 σ A, M1 ⦂ M2 ◎ σ ⊨ A ->
+                       ~ M1 ⦂ M2 ◎ σ ⊭ A) /\
 
-    (forall M1 M2 σ0 σ A, M1 ⦂ M2 ◎ σ0 … σ ⊭ A ->
-                     ~ M1 ⦂ M2 ◎ σ0 … σ ⊨ A).
+    (forall M1 M2 σ A, M1 ⦂ M2 ◎ σ ⊭ A ->
+                       ~ M1 ⦂ M2 ◎ σ ⊨ A).
   Proof.
     apply sat_mutind;
       intros;
@@ -127,79 +56,27 @@ Ltac unique_restriction :=
                  repeat simpl_crush;
                  crush;
                  eauto].
-
-    - (* sat_was *)
-      sat_contra_inversion.
-      + disj_split;
-          subst;
-          match goal with
-          | [H : forall (_ : config), _ -> _ -> _ ⦂ _ ◎ _ … _ ⊭ _,
-               _ : ~ _ ⦂ _ ◎ _ … ?σa ⊭ _ |- _] =>
-            specialize (H σa)
-          end;
-          repeat auto_specialize;
-          auto.
-      + disj_split; subst; auto.
-        match goal with
-        | [H : ~ _ ⦂ _ ⦿ _ ⤳⋆ _  |- _ ] =>
-          contradiction H
-        end.
-        eapply pair_reductions_transitive;
-          eauto.
-
-    - (* sat_in *)
-      sat_contra_inversion.
-      + match goal with
-        | [Ha : forall _, ~ restrict _ _ _,
-             Hb : restrict _ _ ?χ |- _ ] =>
-          specialize (Ha χ);
-            auto
-        end.
-      + unique_restriction;
-          auto.
-
-    - (* nsat_was *)
-      sat_contra_inversion.
-      disj_split;
-        subst;
-        auto.
-      match goal with
-      | [H : ~ _ ⦂ _ ⦿ _ ⤳⋆ _  |- _ ] =>
-        contradiction H
-      end.
-      eapply pair_reductions_transitive;
-        eauto.
-
-    - (* nsat_in *)
-      sat_contra_inversion;
-        unique_restriction;
-        auto.
   Qed.
 
   Theorem sat_implies_not_nsat :
-    (forall M1 M2 σ0 σ A, M1 ⦂ M2 ◎ σ0 … σ ⊨ A ->
-                     ~ M1 ⦂ M2 ◎ σ0 … σ ⊭ A).
+    (forall M1 M2 σ A, M1 ⦂ M2 ◎ σ ⊨ A ->
+                  ~ M1 ⦂ M2 ◎ σ ⊭ A).
   Proof.
     destruct sat_implies_not_nsat_mutind; crush.
   Qed.
 
   Theorem nsat_implies_not_sat :
-    (forall M1 M2 σ0 σ A, M1 ⦂ M2 ◎ σ0 … σ ⊭ A ->
-                     ~ M1 ⦂ M2 ◎ σ0 … σ ⊨ A).
+    (forall M1 M2 σ A, M1 ⦂ M2 ◎ σ ⊭ A ->
+                  ~ M1 ⦂ M2 ◎ σ ⊨ A).
   Proof.
     destruct sat_implies_not_nsat_mutind; crush.
   Qed.
 
-  Fixpoint subst_list {A : Type}`{Subst A nat a_var} (s : list (a_var * nat))(a : A) :=
+  Fixpoint subst_list {A : Type}`{Subst A nat value} (s : list (value * nat))(a : A) :=
     match s with
-    | (x, n) :: s' => ⟦x /s n⟧ (subst_list s' a)
+    | (x, n) :: s' => [x /s n] (subst_list s' a)
     | _ => a
     end.
-
-  Instance substΣavar : Subst a_set nat a_var :=
-    {
-    sbst := sbstΣ
-    }.
 
   Lemma subst_list_asrt_exp :
     forall s e, subst_list s (a_exp e) = (a_exp (subst_list s e)).
@@ -231,7 +108,7 @@ Ltac unique_restriction :=
       try solve [simpl; auto]
     end.
 
-  Fixpoint list_S (s : list (a_var * nat)) :=
+  Fixpoint list_S (s : list (value * nat)) :=
     match s with
     | (a, n) :: s' => (a, S n) :: (list_S s')
     | _ => s
@@ -269,14 +146,14 @@ Ltac unique_restriction :=
   Qed.
 
   Lemma subst_list_all :
-    forall s T A, subst_list s (∀[x⦂ T]∙ A) = (∀[x⦂ T]∙ (subst_list (list_S s) A)).
+    forall s A, subst_list s (∀x.[A]) = (∀x.[(subst_list (list_S s) A)]).
   Proof.
     intro s;
       subst_list_induction.
   Qed.
 
   Lemma subst_list_ex :
-    forall s T A, subst_list s (∃[x⦂ T]∙ A) = (∃[x⦂ T]∙ (subst_list (list_S s) A)).
+    forall s A, subst_list s (∃x.[A]) = (∃x.[(subst_list (list_S s) A)]).
   Proof.
     intro s;
       subst_list_induction.
@@ -290,7 +167,7 @@ Ltac unique_restriction :=
   Qed.
 
   Lemma subst_list_asrt_cons :
-    forall s A x m, (⟦x /s m⟧ subst_list s A) = subst_list ((x, m) :: s) A.
+    forall s A x m, ([x /s m] subst_list s A) = subst_list ((x, m) :: s) A.
   Proof.
     intro s;
       subst_list_induction.
@@ -305,7 +182,7 @@ Ltac unique_restriction :=
 
   Lemma subst_list_calls :
     forall s x y m β, subst_list s (x calls y ◌ m ⟨ β ⟩) =
-                      ((subst_list s x) calls (subst_list s y) ◌ (subst_list s m) ⟨ subst_list s β ⟩).
+                      ((subst_list s x) calls (subst_list s y) ◌ m ⟨ subst_list s β ⟩).
   Proof.
     intro s;
       subst_list_induction.
@@ -325,59 +202,9 @@ Ltac unique_restriction :=
       subst_list_induction.
   Qed.
 
-  Lemma subst_list_next :
-    forall s A, subst_list s (a_next A) = (a_next (subst_list s A)).
-  Proof.
-    intro s;
-      subst_list_induction.
-  Qed.
-
-  Lemma subst_list_will :
-    forall s A, subst_list s (a_will A) = (a_will (subst_list s A)).
-  Proof.
-    intro s;
-      subst_list_induction.
-  Qed.
-
-  Lemma subst_list_prev :
-    forall s A, subst_list s (a_prev A) = (a_prev (subst_list s A)).
-  Proof.
-    intro s;
-      subst_list_induction.
-  Qed.
-
-  Lemma subst_list_was :
-    forall s A, subst_list s (a_was A) = (a_was (subst_list s A)).
-  Proof.
-    intro s;
-      subst_list_induction.
-  Qed.
-
-  Lemma subst_list_in_set :
-    forall s e Σ, subst_list s (a_in e Σ) = a_in (subst_list s e) (subst_list s Σ).
-  Proof.
-    intro s;
-      subst_list_induction.
-  Qed.
-
-  Lemma subst_list_elem :
-    forall s e Σ, subst_list s (e ∈ Σ) = (subst_list s e) ∈ (subst_list s Σ).
-  Proof.
-    intro s;
-      subst_list_induction.
-  Qed.
-
-  Lemma subst_list_self :
-    forall s a', subst_list s (a_self a') = (a_self (subst_list s a')).
-  Proof.
-    intro s;
-      subst_list_induction.
-  Qed.
-
   Ltac subst_list_rewrite :=
     try rewrite subst_list_asrt_exp in *;
     try rewrite subst_list_asrt_class in *;
-    try rewrite subst_list_elem in *;
     try rewrite subst_list_arr in *;
     try rewrite subst_list_and in *;
     try rewrite subst_list_or in *;
@@ -386,19 +213,13 @@ Ltac unique_restriction :=
     try rewrite subst_list_neg in *;
     try rewrite subst_list_access in *;
     try rewrite subst_list_calls in *;
-    try rewrite subst_list_next in *;
-    try rewrite subst_list_will in *;
-    try rewrite subst_list_prev in *;
-    try rewrite subst_list_was in *;
-    try rewrite subst_list_in_set in *;
     try rewrite subst_list_external in *;
-    try rewrite subst_list_internal in *;
-    try rewrite subst_list_self in *.
+    try rewrite subst_list_internal in *.
 
   (** Lemma 5: Classical (1) *)
   Lemma sat_excluded_middle_with_subst :
-    (forall A M1 M2 σ0 σ s, (M1 ⦂ M2 ◎ σ0 … σ ⊨ (subst_list s A)) \/
-                       (M1 ⦂ M2 ◎ σ0 … σ ⊭ (subst_list s A))).
+    (forall A M1 M2 σ s, (M1 ⦂ M2 ◎ σ ⊨ (subst_list s A)) \/
+                    (M1 ⦂ M2 ◎ σ ⊭ (subst_list s A))).
   Proof.
     intro A;
       induction A;
@@ -406,42 +227,30 @@ Ltac unique_restriction :=
       auto;
       subst_list_rewrite;
       try solve [repeat match goal with
-                        | [H : (forall (_ _ : mdl) (_ _ : config)(_ : list (a_var * nat)), _ \/ _)
-                           |- ?M1 ⦂ ?M2 ◎ ?σ0 … ?σ ⊨ _ \/ _ ] =>
-                          specialize (H M1 M2 σ0 σ);
-                          match goal with
-                          | [|- context [subst_list ?s _]] =>
-                            specialize (H s)
-                          end
+                        | [ s' : list (value * nat),
+                                 IH : (forall (_ _ : mdl)(_ : config)(s : list (value * nat)), _) |-
+                            context[?M ⦂ ?M' ◎ ?σ' ⊨ _]] =>
+                          specialize (IH M M' σ' s')
                         end;
-                 repeat match goal with
-                        | [H : _ \/ _ |- _ ] =>
-                          destruct H
-                        end;
-                 eauto with chainmail_db].
+                 repeat disj_split; auto with chainmail_db].
 
     - (* exp *)
       destruct (excluded_middle (exp_satisfaction M1 M2 σ (subst_list s e)));
         auto with chainmail_db.
 
     - (* class *)
-      destruct (excluded_middle (has_class σ (subst_list s a) c));
-        auto with chainmail_db.
-
-    - (* elem *)
-      destruct (excluded_middle (elem_of_set M1 M2 σ (subst_list s e) (subst_list s a)));
+      destruct (excluded_middle (has_class M1 M2 σ (subst_list s e) c));
         auto with chainmail_db.
 
     - (* all *)
-      destruct (excluded_middle (exists x, has_type σ x a /\
-                                      M1 ⦂ M2 ◎ σ0 … σ ⊭ (⟦x /s 0⟧subst_list (list_S s) A)));
+      destruct (excluded_middle (exists x, M1 ⦂ M2 ◎ σ ⊭ ([x /s 0] subst_list (list_S s) A)));
         [destruct_exists_loo;
          andDestruct;
          eauto with chainmail_db|].
       left.
       apply sat_all;
         intros.
-      destruct (IHA M1 M2 σ0 σ ((x, 0)::(list_S s)));
+      destruct (IHA M1 M2 σ ((x, 0)::(list_S s)));
         auto.
       match goal with
       | [ H : ~ _ |- _ ] =>
@@ -450,8 +259,7 @@ Ltac unique_restriction :=
       eauto.
 
     - (* ex *)
-      destruct (excluded_middle (exists x, has_type σ x a /\
-                                           M1 ⦂ M2 ◎ σ0 … σ ⊨ (⟦x /s 0⟧subst_list (list_S s) A)));
+      destruct (excluded_middle (exists x, M1 ⦂ M2 ◎ σ ⊨ ([x /s 0]subst_list (list_S s) A)));
         [destruct_exists_loo;
          andDestruct;
          eauto with chainmail_db|].
@@ -459,7 +267,7 @@ Ltac unique_restriction :=
       right;
         apply nsat_ex;
         intros.
-      destruct (IHA M1 M2 σ0 σ ((x, 0) :: (list_S s)));
+      destruct (IHA M1 M2 σ ((x, 0) :: (list_S s)));
         eauto with chainmail_db.
       match goal with
       | [ H : ~ _ |- _ ] =>
@@ -468,186 +276,96 @@ Ltac unique_restriction :=
       eauto.
 
     - (* access *)
-      destruct (excluded_middle (has_access_aval M1 M2 σ (subst_list s a) (subst_list s a0)));
+      destruct (excluded_middle (has_access σ (subst_list s a) (subst_list s a0)));
         auto with chainmail_db.
 
     - (* calls *)
       destruct (excluded_middle (makes_call σ
                                             (subst_list s a)
                                             (subst_list s a0)
-                                            (subst_list s a1)
+                                            m
                                             (subst_list s p)));
         auto with chainmail_db.
 
-    - (* next *)
-      destruct (excluded_middle (exists σ', M1 ⦂ M2 ⦿ σ ⌈⤳⌉ σ' /\ M1 ⦂ M2 ◎ σ0 … σ' ⊨ (subst_list s A)));
-        [destruct_exists_loo;
-         andDestruct;
-         eauto with chainmail_db
-        |right].
-      apply nsat_next;
-        intros.
-      specialize (IHA M1 M2 σ0 σ' s).
-      disj_split;
-        auto.
-      contradiction n;
-        eauto.
-
-    - (* will *)
-      destruct (excluded_middle (exists σ', M1 ⦂ M2 ⦿ σ ⌈⤳⋆⌉ σ' /\ M1 ⦂ M2 ◎ σ0 … σ' ⊨ (subst_list s A)));
-        [destruct_exists_loo;
-         andDestruct;
-         eauto with chainmail_db
-        |right].
-      apply nsat_will;
-        intros.
-      specialize (IHA M1 M2 σ0 σ' s).
-      disj_split;
-        auto.
-      contradiction n;
-        eauto.
-
-    - (* prev *)
-      destruct (excluded_middle (exists σ', ((M1 ⦂ M2 ⦿ σ0 ⤳⋆ σ' \/
-                                              σ0 = σ') /\
-                                             M1 ⦂ M2 ⦿ σ' ⤳ σ /\
-                                             M1 ⦂ M2 ◎ σ0 … σ' ⊭ (subst_list s A))));
-        [destruct_exists_loo; andDestruct; eauto with chainmail_db|left].
-
-      apply sat_prev;
-        intros.
-      specialize (IHA M1 M2 σ0 σ' s).
-      repeat disj_split;
-        subst;
-        auto;
-        contradiction n;
-        eauto.
-
-    - (* was *)
-      destruct (excluded_middle (M1 ⦂ M2 ⦿ σ0 ⤳⋆ σ));
-        [|auto with chainmail_db].
-      destruct (excluded_middle (exists σ', (M1 ⦂ M2 ⦿ σ0 ⤳⋆ σ' \/
-                                             σ0 = σ') /\
-                                            M1 ⦂ M2 ⦿ σ' ⤳⋆ σ /\
-                                            M1 ⦂ M2 ◎ σ0 … σ' ⊨ (subst_list s A)));
-        [destruct_exists_loo; andDestruct; eauto with chainmail_db|].
-
-      right; apply nsat_was1;
-        intros;
-        auto.
-
-      + specialize (IHA M1 M2 σ0 σ' s).
-        disj_split;
-          eauto with chainmail_db.
-        * contradiction n.
-          exists σ';
-            repeat split;
-            eauto.
-
-      + specialize (IHA M1 M2 σ0 σ0 s).
-        disj_split;
-          eauto with chainmail_db.
-        * contradiction n.
-          exists σ0;
-            repeat split;
-            eauto.
-
-    - (* space *)
-      destruct σ as [χ ψ].
-      destruct (excluded_middle (exists χ', restrict (subst_list s a) χ χ'));
-        [destruct_exists_loo|].
-
-      + specialize (IHA M1 M2 σ0 (χ0, ψ) s);
-          disj_split;
-          eauto with chainmail_db.
-
-      + right; apply nsat_in1;
-          intros; intro Hcontra.
-        contradiction n;
-          eauto.
-
-    - destruct (excluded_middle (external_obj M1 M2 σ (subst_list s a)));
+    - destruct (excluded_middle (external_obj M1 σ (subst_list s a)));
         auto with chainmail_db.
 
-    - destruct (excluded_middle (internal_obj M1 M2 σ (subst_list s a)));
-        auto with chainmail_db.
-
-    - destruct (excluded_middle (is_self σ (subst_list s a)));
+    - destruct (excluded_middle (internal_obj M1 σ (subst_list s a)));
         auto with chainmail_db.
 
   Qed.
 
   Theorem sat_excluded_middle :
-    forall M1 M2 σ0 σ A, M1 ⦂ M2 ◎ σ0 … σ ⊨ A \/
-                         M1 ⦂ M2 ◎ σ0 … σ ⊭ A.
+    forall M1 M2 σ A, M1 ⦂ M2 ◎ σ ⊨ A \/
+                 M1 ⦂ M2 ◎ σ ⊭ A.
   Proof.
     intros.
-    destruct (sat_excluded_middle_with_subst A M1 M2 σ0 σ nil);
+    destruct (sat_excluded_middle_with_subst A M1 M2 σ nil);
       simpl in *;
       auto.
   Qed.
 
   (** Lemma 5: Classical (5) *)
   Lemma arr_true :
-    forall M1 M2 σ0 σ A1 A2,
-      M1 ⦂ M2 ◎ σ0 … σ ⊨ (A1 ⟶ A2) ->
-      M1 ⦂ M2 ◎ σ0 … σ ⊨ A1 ->
-      M1 ⦂ M2 ◎ σ0 … σ ⊨ A2.
+    forall M1 M2 σ A1 A2,
+      M1 ⦂ M2 ◎ σ ⊨ (A1 ⟶ A2) ->
+      M1 ⦂ M2 ◎ σ ⊨ A1 ->
+      M1 ⦂ M2 ◎ σ ⊨ A2.
   Proof.
-    intros M1 M2 σ0 σ A1 A2 Hsat;
+    intros M1 M2 σ A1 A2 Hsat;
       inversion Hsat;
       subst;
       intros;
       auto.
 
-    apply sat_implies_not_nsat_mutind in H4;
+    apply sat_implies_not_nsat_mutind in H3;
       crush.
   Qed.
 
   Lemma arr_false :
-    forall M1 M2 σ0 σ A1 A2,
-      M1 ⦂ M2 ◎ σ0 … σ ⊨ (A1 ⟶ A2) ->
-      M1 ⦂ M2 ◎ σ0 … σ ⊭ A2 ->
-      M1 ⦂ M2 ◎ σ0 … σ ⊭ A1.
+    forall M1 M2 σ A1 A2,
+      M1 ⦂ M2 ◎ σ ⊨ (A1 ⟶ A2) ->
+      M1 ⦂ M2 ◎ σ ⊭ A2 ->
+      M1 ⦂ M2 ◎ σ ⊭ A1.
   Proof.
-    intros M1 M2 σ0 σ A1 A2 Hsat;
+    intros M1 M2 σ A1 A2 Hsat;
       inversion Hsat;
       subst;
       intros;
       auto.
 
-    apply sat_implies_not_nsat_mutind in H4;
+    apply sat_implies_not_nsat_mutind in H3;
       crush.
   Qed.
 
   Lemma arr_prop1 :
-    forall M1 M2 σ0 σ A1 A2,
-      (M1 ⦂ M2 ◎ σ0 … σ ⊨ A1 ->
-       M1 ⦂ M2 ◎ σ0 … σ ⊨ A2) ->
-      M1 ⦂ M2 ◎ σ0 … σ ⊨ (A1 ⟶ A2).
+    forall M1 M2 σ A1 A2,
+      (M1 ⦂ M2 ◎ σ ⊨ A1 ->
+       M1 ⦂ M2 ◎ σ ⊨ A2) ->
+      M1 ⦂ M2 ◎ σ ⊨ (A1 ⟶ A2).
   Proof.
     intros.
     destruct sat_excluded_middle
       with (M1:=M1)(M2:=M2)
-           (σ:=σ)(σ0:=σ0)(A:=A1);
+           (σ:=σ)(A:=A1);
       auto with chainmail_db.
   Qed.
 
   Lemma arr_prop2 :
-    forall M1 M2 σ0 σ A1 A2,
-      M1 ⦂ M2 ◎ σ0 … σ ⊨ (A1 ⟶ A2) ->
-      (M1 ⦂ M2 ◎ σ0 … σ ⊨ A1 ->
-       M1 ⦂ M2 ◎ σ0 … σ ⊨ A2).
+    forall M1 M2 σ A1 A2,
+      M1 ⦂ M2 ◎ σ ⊨ (A1 ⟶ A2) ->
+      (M1 ⦂ M2 ◎ σ ⊨ A1 ->
+       M1 ⦂ M2 ◎ σ ⊨ A2).
   Proof.
     intros.
     eapply arr_true; eauto.
   Qed.
 
   Lemma arr_prop :
-    forall M1 M2 σ0 σ A1 A2,
-      M1 ⦂ M2 ◎ σ0 … σ ⊨ (A1 ⟶ A2) <->
-      (M1 ⦂ M2 ◎ σ0 … σ ⊨ A1 ->
-       M1 ⦂ M2 ◎ σ0 … σ ⊨ A2).
+    forall M1 M2 σ A1 A2,
+      M1 ⦂ M2 ◎ σ ⊨ (A1 ⟶ A2) <->
+      (M1 ⦂ M2 ◎ σ ⊨ A1 ->
+       M1 ⦂ M2 ◎ σ ⊨ A2).
   Proof.
     intros;
       split;
@@ -655,10 +373,9 @@ Ltac unique_restriction :=
   Qed.
 
   Lemma all_x_prop :
-    forall M1 M2 σ0 σ A T,
-      M1 ⦂ M2 ◎ σ0 … σ ⊨ (∀[x⦂ T]∙ A) <->
-      (forall x, has_type σ x T ->
-            M1 ⦂ M2 ◎ σ0 … σ ⊨ (⟦x /s 0⟧A)).
+    forall M1 M2 σ A,
+      M1 ⦂ M2 ◎ σ ⊨ (∀x.[A]) <->
+      (forall x, M1 ⦂ M2 ◎ σ ⊨ ([x /s 0]A)).
   Proof.
     intros; split; eauto with chainmail_db; intros.
     inversion H;
@@ -667,10 +384,9 @@ Ltac unique_restriction :=
   Qed.
 
   Lemma ex_x_prop :
-    forall M1 M2 σ0 σ A T,
-      M1 ⦂ M2 ◎ σ0 … σ ⊨ (∃[x⦂ T]∙A) <->
-      (exists x, has_type σ x T /\
-            M1 ⦂ M2 ◎ σ0 … σ ⊨ (⟦x /s 0⟧ A)).
+    forall M1 M2 σ A,
+      M1 ⦂ M2 ◎ σ ⊨ (∃x.[A]) <->
+      (exists x, M1 ⦂ M2 ◎ σ ⊨ ([x /s 0] A)).
   Proof.
     intros; split; eauto with chainmail_db; intros.
     inversion H;
@@ -683,8 +399,8 @@ Ltac unique_restriction :=
 
   (** Lemma 5: Classical (2) *)
   Lemma and_iff :
-    forall M1 M2 σ0 σ A1 A2, (M1 ⦂ M2 ◎ σ0 … σ ⊨ (A1 ∧ A2)) <->
-                          (M1 ⦂ M2 ◎ σ0 … σ ⊨ A1 /\ M1 ⦂ M2 ◎ σ0 … σ ⊨ A2).
+    forall M1 M2 σ A1 A2, (M1 ⦂ M2 ◎ σ ⊨ (A1 ∧ A2)) <->
+                     (M1 ⦂ M2 ◎ σ ⊨ A1 /\ M1 ⦂ M2 ◎ σ ⊨ A2).
   Proof.
     intros;
       split;
@@ -695,8 +411,8 @@ Ltac unique_restriction :=
 
   (** Lemma 5: Classical (3) *)
   Lemma or_iff :
-    forall M1 M2 σ0 σ A1 A2, (M1 ⦂ M2 ◎ σ0 … σ ⊨ (A1 ∨ A2)) <->
-                        (M1 ⦂ M2 ◎ σ0 … σ ⊨ A1 \/ M1 ⦂ M2 ◎ σ0 … σ ⊨ A2).
+    forall M1 M2 σ A1 A2, (M1 ⦂ M2 ◎ σ ⊨ (A1 ∨ A2)) <->
+                     (M1 ⦂ M2 ◎ σ ⊨ A1 \/ M1 ⦂ M2 ◎ σ ⊨ A2).
   Proof.
     intros;
       split;
@@ -706,71 +422,53 @@ Ltac unique_restriction :=
   Qed.
 
   Lemma negate_elim_sat :
-    (forall A M1 M2 σ0 σ, M1 ⦂ M2 ◎ σ0 … σ ⊨ (¬ ¬ A) ->
-                     M1 ⦂ M2 ◎ σ0 … σ ⊨ A).
+    (forall A M1 M2 σ, M1 ⦂ M2 ◎ σ ⊨ (¬ ¬ A) ->
+                  M1 ⦂ M2 ◎ σ ⊨ A).
   Proof.
     intros;
       auto.
     inversion H;
       subst.
-    inversion H5;
+    inversion H4;
       auto.
   Qed.
 
   Lemma negate_elim_nsat :
-    (forall A M1 M2 σ0 σ, M1 ⦂ M2 ◎ σ0 … σ ⊭ (¬ ¬ A) ->
-                     M1 ⦂ M2 ◎ σ0 … σ ⊭ A).
+    (forall A M1 M2 σ, M1 ⦂ M2 ◎ σ ⊭ (¬ ¬ A) ->
+                  M1 ⦂ M2 ◎ σ ⊭ A).
   Proof.
     intros;
       auto.
     inversion H;
       subst.
-    inversion H5;
+    inversion H4;
       auto.
   Qed.
 
   Lemma negate_intro_sat :
-    (forall A M1 M2 σ0 σ, M1 ⦂ M2 ◎ σ0 … σ ⊨ A ->
-                       M1 ⦂ M2 ◎ σ0 … σ ⊨ (¬ ¬ A)).
+    (forall A M1 M2 σ, M1 ⦂ M2 ◎ σ ⊨ A ->
+                  M1 ⦂ M2 ◎ σ ⊨ (¬ ¬ A)).
   Proof.
     intros;
       auto with chainmail_db.
   Qed.
 
   Lemma negate_intro_nsat :
-    (forall A M1 M2 σ0 σ, M1 ⦂ M2 ◎ σ0 … σ ⊭ A ->
-                     M1 ⦂ M2 ◎ σ0 … σ ⊭ (¬ ¬ A)).
+    (forall A M1 M2 σ, M1 ⦂ M2 ◎ σ ⊭ A ->
+                  M1 ⦂ M2 ◎ σ ⊭ (¬ ¬ A)).
   Proof.
     intros;
       auto with chainmail_db.
   Qed.
 
-  Lemma will_arr :
-    forall M1 M2 σ0 σ A1 A2,
-      M1 ⦂ M2 ◎ σ0 … σ ⊨ a_will(A1 ⟶ A2 ∧ A1) ->
-      M1 ⦂ M2 ◎ σ0 … σ ⊨ a_will(A2).
-  Proof.
-    intros.
-    inversion H;
-      subst.
-    inversion H6;
-      subst;
-      eauto.
-    apply sat_will
-      with (σ':=σ');
-      auto.
-    eapply arr_true;
-      eauto.
-  Qed.
-
   Lemma sat_and_nsat_entails_false :
-    forall A, entails (A ∧ ¬ A) (a_exp (e_val v_false)).
+    forall M A, entails M (A ∧ ¬ A) (a_exp (e_val v_false)).
   Proof.
     intros.
     apply ent;
       intros.
 
-    apply and_iff in H;
+    apply and_iff in H0;
       andDestruct.
     inversion Hb;
       subst.
@@ -782,18 +480,18 @@ Ltac unique_restriction :=
   Hint Resolve sat_and_nsat_entails_false : chainmail_db.
 
   Lemma false_entails_sat_and_nsat :
-    forall A, entails (a_exp (e_val v_false)) (A ∧ ¬ A).
+    forall M A, entails M (a_exp (e_val v_false)) (A ∧ ¬ A).
   Proof.
     intros.
     apply ent;
       intros.
 
-    inversion H;
+    inversion H0;
       subst.
     inversion H5;
       subst.
     match goal with
-    | [H : _ ∙ _ ⊢ _ ↪ _ |- _ ] =>
+    | [H : evaluate _ _ _ _ |- _ ] =>
       inversion H
     end.
   Qed.
@@ -802,7 +500,7 @@ Ltac unique_restriction :=
 
   (** Lemma 6: (1) *)
   Lemma sat_and_nsat_equiv_false :
-    forall A, equiv_a (A ∧ ¬ A) (a_exp (e_val v_false)).
+    forall M A, equiv_a M (A ∧ ¬ A) (a_exp (e_val v_false)).
   Proof.
     intros;
       unfold equiv_a;
@@ -812,13 +510,13 @@ Ltac unique_restriction :=
   Qed.
 
   Lemma or_commutative' :
-    forall A1 A2, entails (A1 ∨ A2) (A2 ∨ A1).
+    forall M A1 A2, entails M (A1 ∨ A2) (A2 ∨ A1).
   Proof.
     intros;
       apply ent;
       intros.
 
-    inversion H;
+    inversion H0;
       eauto with chainmail_db.
   Qed.
 
@@ -826,7 +524,7 @@ Ltac unique_restriction :=
 
   (** Lemma 6: (4) *)
   Lemma or_commutative :
-    forall A1 A2, equiv_a (A1 ∨ A2) (A2 ∨ A1).
+    forall M A1 A2, equiv_a M (A1 ∨ A2) (A2 ∨ A1).
   Proof.
     intros;
       unfold equiv_a;
@@ -838,13 +536,13 @@ Ltac unique_restriction :=
   Hint Resolve or_commutative : chainmail_db.
 
   Lemma and_commutative' :
-    forall A1 A2, entails (A1 ∧ A2) (A2 ∧ A1).
+    forall M A1 A2, entails M (A1 ∧ A2) (A2 ∧ A1).
   Proof.
     intros;
       eapply ent;
       intros;
       eauto.
-    inversion H;
+    inversion H0;
       eauto with chainmail_db.
   Qed.
 
@@ -852,7 +550,7 @@ Ltac unique_restriction :=
 
   (** Lemma 6: (3) *)
   Lemma and_commutative :
-    forall A1 A2, equiv_a (A1 ∧ A2) (A2 ∧ A1).
+    forall M A1 A2, equiv_a M (A1 ∧ A2) (A2 ∧ A1).
   Proof.
     intros;
       unfold equiv_a;
@@ -864,12 +562,12 @@ Ltac unique_restriction :=
   Hint Resolve and_commutative : chainmail_db.
 
   Lemma or_associative_1:
-    forall A1 A2 A3, entails ((A1 ∨ A2) ∨ A3) (A1 ∨ (A2 ∨ A3)).
+    forall M A1 A2 A3, entails M ((A1 ∨ A2) ∨ A3) (A1 ∨ (A2 ∨ A3)).
   Proof.
     intros;
       apply ent;
       intros;
-      inversion H;
+      inversion H0;
       subst;
       eauto;
       inversion H5;
@@ -879,12 +577,12 @@ Ltac unique_restriction :=
   Hint Resolve or_associative_1 : chainmail_db.
 
   Lemma or_associative_2:
-    forall A1 A2 A3, entails (A1 ∨ (A2 ∨ A3)) ((A1 ∨ A2) ∨ A3).
+    forall M A1 A2 A3, entails M (A1 ∨ (A2 ∨ A3)) ((A1 ∨ A2) ∨ A3).
   Proof.
     intros;
       apply ent;
       intros;
-      inversion H;
+      inversion H0;
       subst;
       eauto;
       inversion H5;
@@ -895,7 +593,7 @@ Ltac unique_restriction :=
 
   (** Lemma 6: (5) *)
   Lemma or_associative:
-    forall A1 A2 A3, equiv_a ((A1 ∨ A2) ∨ A3) (A1 ∨ (A2 ∨ A3)).
+    forall M A1 A2 A3, equiv_a M ((A1 ∨ A2) ∨ A3) (A1 ∨ (A2 ∨ A3)).
   Proof.
     intros;
       unfold equiv_a;
@@ -907,12 +605,12 @@ Ltac unique_restriction :=
   Hint Resolve or_associative : chainmail_db.
 
   Lemma and_distributive_1:
-    forall A1 A2 A3, entails ((A1 ∨ A2) ∧ A3) ((A1 ∧ A3) ∨ (A2 ∧ A3)).
+    forall M A1 A2 A3, entails M ((A1 ∨ A2) ∧ A3) ((A1 ∧ A3) ∨ (A2 ∧ A3)).
   Proof.
     intros;
       apply ent;
       intros;
-      inversion H;
+      inversion H0;
       subst;
       eauto;
       inversion H6;
@@ -922,12 +620,12 @@ Ltac unique_restriction :=
   Hint Resolve and_distributive_1 : chainmail_db.
 
   Lemma and_distributive_2:
-    forall A1 A2 A3, entails ((A1 ∧ A3) ∨ (A2 ∧ A3)) ((A1 ∨ A2) ∧ A3).
+    forall M A1 A2 A3, entails M ((A1 ∧ A3) ∨ (A2 ∧ A3)) ((A1 ∨ A2) ∧ A3).
   Proof.
     intros;
       apply ent;
       intros;
-      inversion H;
+      inversion H0;
       subst;
       eauto;
       inversion H5;
@@ -938,7 +636,7 @@ Ltac unique_restriction :=
 
   (** Lemma 6: (6) *)
   Lemma and_distributive:
-    forall A1 A2 A3, equiv_a ((A1 ∨ A2) ∧ A3) ((A1 ∧ A3) ∨ (A2 ∧ A3)).
+    forall M A1 A2 A3, equiv_a M ((A1 ∨ A2) ∧ A3) ((A1 ∧ A3) ∨ (A2 ∧ A3)).
   Proof.
     intros;
       unfold equiv_a;
@@ -950,12 +648,12 @@ Ltac unique_restriction :=
   Hint Resolve and_distributive : chainmail_db.
 
   Lemma or_distributive_1:
-    forall A1 A2 A3, entails ((A1 ∧ A2) ∨ A3) ((A1 ∨ A3) ∧ (A2 ∨ A3)).
+    forall M A1 A2 A3, entails M ((A1 ∧ A2) ∨ A3) ((A1 ∨ A3) ∧ (A2 ∨ A3)).
   Proof.
     intros;
       apply ent;
       intros;
-      inversion H;
+      inversion H0;
       subst;
       eauto with chainmail_db;
       inversion H5;
@@ -965,12 +663,12 @@ Ltac unique_restriction :=
   Hint Resolve or_distributive_1 : chainmail_db.
 
   Lemma or_distributive_2:
-    forall A1 A2 A3, entails ((A1 ∨ A3) ∧ (A2 ∨ A3)) ((A1 ∧ A2) ∨ A3).
+    forall M A1 A2 A3, entails M ((A1 ∨ A3) ∧ (A2 ∨ A3)) ((A1 ∧ A2) ∨ A3).
   Proof.
     intros;
       apply ent;
       intros;
-      inversion H;
+      inversion H0;
       subst;
       eauto;
       inversion H6;
@@ -982,7 +680,7 @@ Ltac unique_restriction :=
 
   (** Lemma 6: (7) *)
   Lemma or_distributive:
-    forall A1 A2 A3, equiv_a ((A1 ∧ A2) ∨ A3) ((A1 ∨ A3) ∧ (A2 ∨ A3)).
+    forall M A1 A2 A3, equiv_a M ((A1 ∧ A2) ∨ A3) ((A1 ∨ A3) ∧ (A2 ∨ A3)).
   Proof.
     intros;
       unfold equiv_a;
@@ -994,12 +692,12 @@ Ltac unique_restriction :=
   Hint Resolve or_distributive : chainmail_db.
 
   Lemma neg_distributive_and_1:
-    forall A1 A2, entails (¬(A1 ∧ A2))  (¬A1 ∨ ¬A2).
+    forall M A1 A2, entails M (¬(A1 ∧ A2))  (¬A1 ∨ ¬A2).
   Proof.
     intros;
       apply ent;
       intros;
-      inversion H;
+      inversion H0;
       subst;
       eauto;
       inversion H5;
@@ -1009,12 +707,12 @@ Ltac unique_restriction :=
   Hint Resolve neg_distributive_and_1 : chainmail_db.
 
   Lemma neg_distributive_and_2:
-    forall A1 A2, entails (¬A1 ∨ ¬A2) (¬(A1 ∧ A2)).
+    forall M A1 A2, entails M (¬A1 ∨ ¬A2) (¬(A1 ∧ A2)).
   Proof.
     intros;
       apply ent;
       intros;
-      inversion H;
+      inversion H0;
       subst;
       eauto;
       inversion H5;
@@ -1025,7 +723,7 @@ Ltac unique_restriction :=
 
   (** Lemma 6: (8) *)
   Lemma neg_distributive_and:
-    forall A1 A2, equiv_a (¬(A1 ∧ A2))  (¬A1 ∨ ¬A2).
+    forall M A1 A2, equiv_a M (¬(A1 ∧ A2))  (¬A1 ∨ ¬A2).
   Proof.
     intros;
       unfold equiv_a;
@@ -1037,12 +735,12 @@ Ltac unique_restriction :=
   Hint Resolve neg_distributive_and : chainmail_db.
 
   Lemma neg_distributive_or_1:
-    forall A1 A2, entails (¬(A1 ∨ A2)) (¬A1 ∧ ¬A2).
+    forall M A1 A2, entails M (¬(A1 ∨ A2)) (¬A1 ∧ ¬A2).
   Proof.
     intros;
       apply ent;
       intros;
-      inversion H;
+      inversion H0;
       subst;
       eauto;
       inversion H5;
@@ -1052,12 +750,12 @@ Ltac unique_restriction :=
   Hint Resolve neg_distributive_or_1 : chainmail_db.
 
   Lemma neg_distributive_or_2:
-    forall A1 A2, entails (¬A1 ∧ ¬A2) (¬(A1 ∨ A2)).
+    forall M A1 A2, entails M (¬A1 ∧ ¬A2) (¬(A1 ∨ A2)).
   Proof.
     intros;
       apply ent;
       intros;
-      inversion H;
+      inversion H0;
       subst;
       eauto;
       inversion H6;
@@ -1069,7 +767,7 @@ Ltac unique_restriction :=
 
   (** Lemma 6: (9) *)
   Lemma neg_distributive_or:
-    forall A1 A2, equiv_a (¬(A1 ∨ A2)) (¬A1 ∧ ¬A2).
+    forall M A1 A2, equiv_a M (¬(A1 ∨ A2)) (¬A1 ∧ ¬A2).
   Proof.
     intros;
       unfold equiv_a;
@@ -1081,13 +779,13 @@ Ltac unique_restriction :=
   Hint Resolve neg_distributive_or : chainmail_db.
 
   Lemma not_ex_x_all_not_1 : 
-    forall A T, entails (¬(∃[x⦂ T]∙A)) (∀[x⦂ T]∙¬A).
+    forall M A, entails M (¬(∃x.[A])) (∀x.[¬A]).
   Proof.
     intros;
       apply ent;
       intros.
 
-    inversion H;
+    inversion H0;
       subst.
     inversion H5;
       subst.
@@ -1101,30 +799,36 @@ Ltac unique_restriction :=
   Hint Resolve not_ex_x_all_not_1 : chainmail_db.
 
   Lemma not_ex_x_all_not_2 : 
-    forall A T, entails (∀[x⦂ T]∙¬A) (¬(∃[x⦂ T]∙A)).
+    forall M A, entails M (∀x.[¬A]) (¬(∃x.[A])).
   Proof.
     intros;
       apply ent;
       intros.
 
-    inversion H;
+    inversion H0;
       subst.
 
     apply sat_not.
     apply nsat_ex;
       intros.
-    eapply H5 in H0;
-      eauto with chainmail_db.
+    match goal with
+    | [H : forall _, _ |- context[[?x' /s _ ] _]] =>
+      specialize (H x')
+    end.
 
-    inversion H0;
-      eauto with chainmail_db.
+    subst_simpl.
+    match goal with
+    | [H : _ ⦂ _ ◎ _ ⊨ ¬ _ |- _ ] =>
+      inversion H;
+        auto
+    end.
   Qed.
 
   Hint Resolve not_ex_x_all_not_2 : chainmail_db.
 
   (** Lemma 6: (10) *)
   Lemma not_ex_x_all_not : 
-    forall A T, equiv_a (¬(∃[x⦂ T]∙A)) (∀[x⦂ T]∙¬A).
+    forall M A, equiv_a M (¬(∃x.[A])) (∀x.[¬A]).
   Proof.
     intros;
       unfold equiv_a;
@@ -1136,13 +840,13 @@ Ltac unique_restriction :=
   Hint Resolve not_ex_x_all_not : chainmail_db.
 
   Lemma not_all_x_ex_not_1 : 
-    forall A T, entails (¬(∀[x⦂ T]∙A)) (∃[x⦂ T]∙¬A).
+    forall M A, entails M (¬(∀x.[A])) (∃x.[¬A]).
   Proof.
     intros;
       apply ent;
       intros.
 
-    inversion H;
+    inversion H0;
       subst.
     inversion H5;
       subst.
@@ -1156,25 +860,25 @@ Ltac unique_restriction :=
   Hint Resolve not_all_x_ex_not_1 : chainmail_db.
 
   Lemma not_all_x_ex_not_2 : 
-    forall A T, entails (∃[x⦂ T]∙¬A) (¬(∀[x⦂ T]∙A)).
+    forall M A, entails M (∃x.[¬A]) (¬(∀x.[A])).
   Proof.
     intros;
       apply ent;
       intros.
 
-    inversion H;
+    inversion H0;
       subst.
 
     apply sat_not.
     apply nsat_all with (x:=x);
       auto with chainmail_db.
-    inversion H7; subst; auto.
+    inversion H5; subst; auto.
   Qed.
 
   Hint Resolve not_all_x_ex_not_2 : chainmail_db.
 
   Lemma not_all_x_ex_not : 
-    forall A T, equiv_a (¬(∀[x⦂ T]∙A)) (∃[x⦂ T]∙¬A).
+    forall M A, equiv_a M (¬(∀x.[A])) (∃x.[¬A]).
   Proof.
     intros;
       unfold equiv_a;
@@ -1186,9 +890,10 @@ Ltac unique_restriction :=
   Hint Resolve not_all_x_ex_not : chainmail_db.
 
   Lemma entails_implies :
-    forall {M1 M2 σ0 σ A1 A2}, entails A1 A2 ->
-                          M1 ⦂ M2 ◎ σ0 … σ ⊨ A1 ->
-                          M1 ⦂ M2 ◎ σ0 … σ ⊨ A2.
+    forall {M1 M2 σ A1 A2}, entails M1 A1 A2 ->
+                       arising M1 M2  σ ->
+                       M1 ⦂ M2 ◎ σ ⊨ A1 ->
+                       M1 ⦂ M2 ◎ σ ⊨ A2.
   Proof.
     intros.
     inversion H;
@@ -1199,8 +904,8 @@ Ltac unique_restriction :=
 
   Ltac a_intro :=
     match goal with
-    | [|- _ ⦂ _ ◎ _ … _ ⊨ (∀[x⦂ _ ]∙ _)] => apply sat_all; intros; simpl in *
-    | [|- _ ⦂ _ ◎ _ … _ ⊨ (_ ⟶ _)] => apply arr_prop1; intros; simpl in *
+    | [|- _ ⦂ _ ◎ _ ⊨ (∀x.[ _])] => apply sat_all; intros; simpl in *
+    | [|- _ ⦂ _ ◎ _ ⊨ (_ ⟶ _)] => apply arr_prop1; intros; simpl in *
     end.
 
   Ltac a_intros :=
@@ -1208,25 +913,25 @@ Ltac unique_restriction :=
 
   Ltac a_prop :=
     repeat match goal with
-           | [H : _ ⦂ _ ◎ _ … _ ⊨ (_ ∧ _) |- _] => apply -> and_iff in H;
+           | [H : _ ⦂ _ ◎ _ ⊨ (_ ∧ _) |- _] => apply -> and_iff in H;
                                                destruct H
-           | [H : _ ⦂ _ ◎ _ … _ ⊨ (_ ∨ _) |- _] => apply -> or_iff in H
-           | [H : _ ⦂ _ ◎ _ … _ ⊨ (_ ⟶ _) |- _] => rewrite -> arr_prop in H
-           | [H : context[_ ⦂ _ ◎ _ … _ ⊨ (_ ⟶ _)] |- _] => rewrite -> arr_prop in H
-           | [H : _ ⦂ _ ◎ _ … _ ⊨ (∀[x⦂ _]∙_) |- _] => rewrite all_x_prop in H; simpl in *
-           | [|- _ ⦂ _ ◎ _ … _ ⊨ (_ ∧ _)] => apply sat_and
-           | [|- _ ⦂ _ ◎ _ … _ ⊨ (_ ∨ _)] => apply <- or_iff
+           | [H : _ ⦂ _ ◎ _ ⊨ (_ ∨ _) |- _] => apply -> or_iff in H
+           | [H : _ ⦂ _ ◎ _ ⊨ (_ ⟶ _) |- _] => rewrite -> arr_prop in H
+           | [H : context[_ ⦂ _ ◎ _ ⊨ (_ ⟶ _)] |- _] => rewrite -> arr_prop in H
+           | [H : _ ⦂ _ ◎ _ ⊨ (∀x.[_]) |- _] => rewrite all_x_prop in H; simpl in *
+           | [|- _ ⦂ _ ◎ _ ⊨ (_ ∧ _)] => apply sat_and
+           | [|- _ ⦂ _ ◎ _ ⊨ (_ ∨ _)] => apply <- or_iff
            | [H : entails ?A1 ?A2,
-                  Ha : ?M1 ⦂ ?M2 ◎  ?σ0 … (?χ, ?ϕ::?ψ) ⊨ ?A1 |- _] =>
-             notHyp (M1 ⦂ M2 ◎ σ0 … (χ, ϕ::ψ) ⊨ A2);
+                  Ha : ?M1 ⦂ ?M2 ◎  (?χ, ?ϕ::?ψ) ⊨ ?A1 |- _] =>
+             notHyp (M1 ⦂ M2 ◎ (χ, ϕ::ψ) ⊨ A2);
              let H' := fresh in 
-             assert (H' : M1 ⦂ M2 ◎ σ0 … (χ, ϕ::ψ) ⊨ A2);
+             assert (H' : M1 ⦂ M2 ◎ (χ, ϕ::ψ) ⊨ A2);
              [apply (entails_implies M1 M2 χ ϕ ψ A1 Ha A2 H); eauto|]
-           | [Ha : ?M1 ⦂ ?M2 ◎  ?σ0 … ?σ ⊨ ?A,
-                   Hb : ?M1 ⦂ ?M2 ◎ ?σ0 … ?σ ⊨ ¬ ?A |- _] =>
+           | [Ha : ?M1 ⦂ ?M2 ◎  ?σ ⊨ ?A,
+                   Hb : ?M1 ⦂ ?M2 ◎ ?σ ⊨ ¬ ?A |- _] =>
              apply sat_implies_not_nsat in Ha
-           | [Ha : ?M1 ⦂ ?M2 ◎ ?σ0 … ?σ ⊨ ¬ ?A,
-                   Hb : ~ ?M1 ⦂ ?M2 ◎ ?σ0 … ?σ ⊭ ?A |- _] =>
+           | [Ha : ?M1 ⦂ ?M2 ◎ ?σ ⊨ ¬ ?A,
+                   Hb : ~ ?M1 ⦂ ?M2 ◎ ?σ ⊭ ?A |- _] =>
              inversion Ha; subst; crush
            end.
 
