coq_inference/chainmail_tactics.v
@@ -4,15 +4,15 @@ Require Import L_def.
 Require Import exp.
 Require Import defs.
 Require Import operational_semantics.
-Require Import inference.
+Require Import chainmail.
 Require Import List.
 Require Export Coq.Lists.ListSet.
 
 Module ChainmailTactics(L : LanguageDef).
 
   Import L.
-  Module L_Inference := Inference(L).
-  Export L_Inference.
+  Module L_Chainmail := Chainmail(L).
+  Export L_Chainmail.
 
   Open Scope chainmail_scope.
   Declare Scope chainmail_tactics_scope.
@@ -549,102 +549,5 @@ Module ChainmailTactics(L : LanguageDef).
     repeat extract_from_map v' n';
     repeat extract_from_asrt v';
     subst.
-
-  Open Scope inference_scope.
-
-  Ltac extract1 v' n' :=
-    match goal with
-    | [|- ?M ⊢ _ to1 ?A2 onlyIf ?A3] =>
-      let A2' := fresh "A" in
-      let H2 := fresh in
-      let A3' := fresh "A" in
-      let H3 := fresh in
-      remember A2 as A2'  eqn : H2;
-      remember A3 as A3'  eqn : H3;
-      extract v' n';
-      subst A2' A3'
-    | [|- ?M ⊢ _ to ?A2 onlyIf ?A3] =>
-      let A2' := fresh "A" in
-      let H2 := fresh in
-      let A3' := fresh "A" in
-      let H3 := fresh in
-      remember A2 as A2'  eqn : H2;
-      remember A3 as A3'  eqn : H3;
-      extract v' n';
-      subst A2' A3'
-    | [|- ?M ⊢ _ to ?A2 onlyThrough ?A3] =>
-      let A2' := fresh "A" in
-      let H2 := fresh in
-      let A3' := fresh "A" in
-      let H3 := fresh in
-      remember A2 as A2'  eqn : H2;
-      remember A3 as A3'  eqn : H3;
-      extract v' n';
-      subst A2' A3'
-    end.
-
-  Ltac extract2 v' n' :=
-    match goal with
-    | [|- ?M ⊢ ?A1 to1 _ onlyIf ?A3] =>
-      let A1' := fresh "A" in
-      let H1 := fresh in
-      let A3' := fresh "A" in
-      let H3 := fresh in
-      remember A1 as A1'  eqn : H1;
-      remember A3 as A3'  eqn : H3;
-      extract v' n';
-      subst A1' A3
-    | [|- ?M ⊢ ?A1 to _ onlyIf ?A3] =>
-      let A1' := fresh "A" in
-      let H1 := fresh in
-      let A3' := fresh "A" in
-      let H3 := fresh in
-      remember A1 as A1'  eqn : H1;
-      remember A3 as A3'  eqn : H3;
-      extract v' n';
-      subst A1' A3
-    | [|- ?M ⊢ ?A1 to _ onlyThrough ?A3] =>
-      let A1' := fresh "A" in
-      let H1 := fresh in
-      let A3' := fresh "A" in
-      let H3 := fresh in
-      remember A1 as A1'  eqn : H1;
-      remember A3 as A3'  eqn : H3;
-      extract v' n';
-      subst A1' A3'
-    end.
-
-  Ltac extract3 v' n' :=
-    match goal with
-    | [|- ?M ⊢ ?A1 to1 ?A2 onlyIf _] =>
-      let A1' := fresh "A" in
-      let H1 := fresh in
-      let A2' := fresh "A" in
-      let H2 := fresh in
-      remember A1 as A1'  eqn : H1;
-      remember A2 as A2'  eqn : H2;
-      extract v' n';
-      subst
-
-    | [|- ?M ⊢ ?A1 to ?A2 onlyIf _] =>
-      let A1' := fresh "A" in
-      let H1 := fresh in
-      let A2' := fresh "A" in
-      let H2 := fresh in
-      remember A1 as A1'  eqn : H1;
-      remember A2 as A2'  eqn : H2;
-      extract v' n';
-      subst A1' A2'
-
-    | [|- ?M ⊢ ?A1 to ?A2 onlyThrough _] =>
-      let A1' := fresh "A" in
-      let H1 := fresh in
-      let A2' := fresh "A" in
-      let H2 := fresh in
-      remember A1 as A1'  eqn : H1;
-      remember A2 as A2'  eqn : H2;
-      extract v' n';
-      subst A1' A2'
-    end.
 
 End ChainmailTactics.
