coq_inference/inference.v
@@ -27,7 +27,7 @@ Module Inference(L : LanguageDef).
 
   Lemma caller_ext :
     forall M α1 α2 m β, M ⊢ α1 calls α2 ◌ m ⟨ β ⟩ ⊇ α1 external.
-    Admitted.
+  Admitted.
 
   Lemma calls_recv :
     forall M α1 α2 m β, M ⊢ α1 calls α2 ◌ m ⟨ β ⟩ ⊇ α1 access α2.
@@ -45,14 +45,14 @@ Module Inference(L : LanguageDef).
 
   Lemma inside_wrapped :
     forall M α C Def, ⟦ C ↦ Def ⟧_∈ M ->
-                 annot Def = inside ->
-                 M ⊢ a_class (e_addr α) C ⊇ wrapped (a_ α).
+                      annot Def = inside ->
+                      M ⊢ a_class (e_addr α) C ⊇ wrapped (a_ α).
   Admitted.
 
   Lemma fld_type :
     forall M e C CDef f D, ⟦ C ↦ CDef ⟧_∈ M ->
-                      ⟦ f ↦ (t_cls D) ⟧_∈ c_fields CDef ->
-                      M ⊢ a_class e C ⊇ a_class ((e_acc_f e f)) D.
+                           ⟦ f ↦ (t_cls D) ⟧_∈ c_fields CDef ->
+                           M ⊢ a_class e C ⊇ a_class ((e_acc_f e f)) D.
   Admitted.
 
   Lemma absurd :
@@ -69,8 +69,8 @@ Module Inference(L : LanguageDef).
 
   Lemma consequence_transitivity :
     forall M A1 A2 A3, M ⊢ A1 ⊇ A2 ->
-                  M ⊢ A2 ⊇ A3 ->
-                  M ⊢ A1 ⊇ A3.
+                       M ⊢ A2 ⊇ A3 ->
+                       M ⊢ A1 ⊇ A3.
   Admitted.
 
   Inductive intrnl : mdl -> asrt -> exp -> Prop :=
@@ -79,61 +79,65 @@ Module Inference(L : LanguageDef).
   | i_false : forall M A, intrnl M A (e_false)
   | i_null : forall M A, intrnl M A (e_null)
   | i_obj : forall M A α C, M ⊢ A ⊇ (a_class (e_addr α) C) ->
-                       C ∈ M ->
-                       intrnl M A (e_addr α)
-  | i_var : forall M A x C, M ⊢ A ⊇ (a_class (e_var x) C) ->
-                       C ∈ M ->
-                       intrnl M A (e_var x)
+                            C ∈ M ->
+                            intrnl M A (e_addr α)
+(*  | i_var : forall M A x C, M ⊢ A ⊇ (a_class (e_var x) C) ->
+                            C ∈ M ->
+                            intrnl M A (e_var x)*)
   | i_fld : forall M A e C CDef f D, intrnl M A e ->
-                                M ⊢ A ⊇ (a_class e C) ->
-                                ⟦ C ↦ CDef ⟧_∈ M ->
-                                ⟦ f ↦ (t_cls D) ⟧_∈ c_fields CDef ->
-                                D ∈ M ->
-                                intrnl M A (e_acc_f e f)
+                                     M ⊢ A ⊇ (a_class e C) ->
+                                     ⟦ C ↦ CDef ⟧_∈ M ->
+                                     ⟦ f ↦ (t_cls D) ⟧_∈ c_fields CDef ->
+                                     D ∈ M ->
+                                     intrnl M A (e_acc_f e f)
   | i_ghost : forall M A e1 e2 C CDef e g, intrnl M A e1 ->
-                                      intrnl M A e2 ->
-                                      M ⊢ A ⊇ (a_class e1 C) ->
-                                      ⟦ C ↦ CDef ⟧_∈ M ->
-                                      ⟦ g ↦ (int, e) ⟧_∈ c_g_fields CDef ->
-                                      intrnl M A (e_acc_g e1 g e2).
+                                           intrnl M A e2 ->
+                                           M ⊢ A ⊇ (a_class e1 C) ->
+                                           ⟦ C ↦ CDef ⟧_∈ M ->
+                                           ⟦ g ↦ (int, e) ⟧_∈ c_g_fields CDef ->
+                                           intrnl M A (e_acc_g e1 g e2).
+
+  Hint Constructors intrnl : inference_db.
 
   Inductive enc : mdl -> asrt -> asrt -> Prop :=
   | enc_intrnl : forall M A e, intrnl M A e ->
-                          enc M A (a_exp e)
+                               enc M A (a_exp e)
   | enc_field : forall M A e f, intrnl M A e ->
-                           enc M A (a_exp (e_acc_f e f))
+                                enc M A (a_exp (e_acc_f e f))
   | enc_int_acc : forall M A α1 α2, M ⊢ A ⊇ (α1 internal) ->
-                               enc M A (α1 access α2)
+                                    enc M A (α1 access α2)
   | enc_wrapped1 : forall M A α, enc M A (wrapped α)
   | enc_wrapped2 : forall M A α1 α2, M ⊢ A ⊇ (wrapped α2) ->
-                                enc M A (¬ α1 access α2)
+                                     enc M A (¬ α1 access α2)
   | enc_conseq : forall M A1 A2 A, M ⊢ A1 ⊇ A2 ->
-                              enc M A2 A ->
-                              enc M A1 A.
+                                   enc M A2 A ->
+                                   enc M A1 A.
+
+  Hint Constructors enc : inference_db.
 
   Inductive only_if : mdl -> asrt -> asrt -> asrt -> Prop :=
   | if_start  : forall M A1 A2 A, M ⊢ A1 ⊇ A ->
-                             M ⊢ A1 to A2 onlyIf A
+                                  M ⊢ A1 to A2 onlyIf A
   | if_conseq : forall M A1 A1' A2 A2' A A', M ⊢ A1' to A2' onlyIf A' ->
-                                        M ⊢ A1 ⊇ A1' ->
-                                        M ⊢ A2 ⊇ A2' ->
-                                        M ⊢ A' ⊇ A ->
-                                        M ⊢ A1 to A2 onlyIf A
+                                             M ⊢ A1 ⊇ A1' ->
+                                             M ⊢ A2 ⊇ A2' ->
+                                             M ⊢ A' ⊇ A ->
+                                             M ⊢ A1 to A2 onlyIf A
   | if_orI1   : forall M A1 A1' A2 A A', M ⊢ A1 to A2 onlyIf A ->
-                                    M ⊢ A1' to A2 onlyIf A' ->
-                                    M ⊢ A1 ∨ A1' to A2 onlyIf A ∨ A'
+                                         M ⊢ A1' to A2 onlyIf A' ->
+                                         M ⊢ A1 ∨ A1' to A2 onlyIf A ∨ A'
   | if_orI2   : forall M A1 A2 A2' A A', M ⊢ A1 to A2 onlyIf A ->
-                                    M ⊢ A1 to A2' onlyIf A' ->
-                                    M ⊢ A1 to A2 ∨ A2' onlyIf A ∨ A'
+                                         M ⊢ A1 to A2' onlyIf A' ->
+                                         M ⊢ A1 to A2 ∨ A2' onlyIf A ∨ A'
   | if_orE    : forall M A1 A2 A A', M ⊢ A1 to A2 onlyIf A ∨ A' ->
-                                M ⊢ A' to A2 onlyThrough a_exp (e_false) ->
-                                M ⊢ A1 to A2 onlyIf A
+                                     M ⊢ A' to A2 onlyThrough a_exp (e_false) ->
+                                     M ⊢ A1 to A2 onlyIf A
   | if_andI : forall M A1 A2 A A', M ⊢ A1 to A2 onlyIf A ->
-                              M ⊢ A1 to A2 onlyIf A' ->
-                              M ⊢ A1 to A2 onlyIf A ∧ A'
+                                   M ⊢ A1 to A2 onlyIf A' ->
+                                   M ⊢ A1 to A2 onlyIf A ∧ A'
   | if_trans  : forall M A1 A2 A A', M ⊢ A1 to A2 onlyThrough A' ->
-                                M ⊢ A1 to A' onlyIf A ->
-                                M ⊢ A1 to A2 onlyIf A
+                                     M ⊢ A1 to A' onlyIf A ->
+                                     M ⊢ A1 to A2 onlyIf A
 
   where
   "M '⊢' A1 'to' A2 'onlyIf' A3" := (only_if M A1 A2 A3)
@@ -141,35 +145,33 @@ Module Inference(L : LanguageDef).
   with only_through : mdl -> asrt -> asrt -> asrt -> Prop :=
   | ot_end      : forall M A1 A2, M ⊢ A1 to A2 onlyThrough A2
   | ot_if       : forall M A1 A2 A, M ⊢ A1 to A2 onlyIf A ->
-                               M ⊢ A1 to A2 onlyThrough A
-  | ot_changes  : forall M A A', M ⊢ A to1 ¬ A onlyIf A' ->
-                            M ⊢ A to ¬ A onlyThrough A'
+                                    M ⊢ A1 to A2 onlyThrough A
   | ot_conseq   : forall M A1 A1' A2 A2' A A', M ⊢ A1' to A2' onlyThrough A' ->
-                                          M ⊢ A1 ⊇ A1' ->
-                                          M ⊢ A2 ⊇ A2' ->
-                                          M ⊢ A' ⊇ A ->
-                                          M ⊢ A1 to A2 onlyThrough A
+                                               M ⊢ A1 ⊇ A1' ->
+                                               M ⊢ A2 ⊇ A2' ->
+                                               M ⊢ A' ⊇ A ->
+                                               M ⊢ A1 to A2 onlyThrough A
   | ot_orI1     : forall M A1 A1' A2 A A', M ⊢ A1 to A2 onlyThrough A ->
-                                      M ⊢ A1' to A2 onlyThrough A' ->
-                                      M ⊢ A1 ∨ A1' to A2 onlyThrough A ∨ A'
+                                           M ⊢ A1' to A2 onlyThrough A' ->
+                                           M ⊢ A1 ∨ A1' to A2 onlyThrough A ∨ A'
   | ot_orI2     : forall M A1 A2 A2' A A', M ⊢ A1 to A2 onlyThrough A ->
-                                      M ⊢ A1 to A2' onlyThrough A' ->
-                                      M ⊢ A1 to A2 ∨ A2 onlyThrough A ∨ A'
+                                           M ⊢ A1 to A2' onlyThrough A' ->
+                                           M ⊢ A1 to A2 ∨ A2 onlyThrough A ∨ A'
   | ot_orE1     : forall M A1 A2 A A', M ⊢ A1 to A2 onlyThrough A ∨ A' ->
-                                  M ⊢ A1 to A' onlyThrough a_exp (e_false) ->
-                                  M ⊢ A1 to A2 onlyThrough A
+                                       M ⊢ A1 to A' onlyThrough a_exp (e_false) ->
+                                       M ⊢ A1 to A2 onlyThrough A
   | ot_orE2     : forall M A1 A2 A A', M ⊢ A1 to A2 onlyThrough A ∨ A' ->
-                                  M ⊢ A' to A2 onlyThrough a_exp (e_false) ->
-                                  M ⊢ A1 to A2 onlyThrough A
+                                       M ⊢ A' to A2 onlyThrough a_exp (e_false) ->
+                                       M ⊢ A1 to A2 onlyThrough A
   | ot_trans1   : forall M A1 A2 A A', M ⊢ A1 to A2 onlyThrough A' ->
-                                  M ⊢ A1 to A' onlyThrough A ->
-                                  M ⊢ A1 to A2 onlyThrough A
+                                       M ⊢ A1 to A' onlyThrough A ->
+                                       M ⊢ A1 to A2 onlyThrough A
   | ot_trans2   : forall M A1 A2 A A', M ⊢ A1 to A2 onlyThrough A' ->
-                                  M ⊢ A' to A2 onlyThrough A ->
-                                  M ⊢ A1 to A2 onlyThrough A
+                                       M ⊢ A' to A2 onlyThrough A ->
+                                       M ⊢ A1 to A2 onlyThrough A
   | ot_inv      : forall M A1 A2 A3 A, M ⊢ A to ¬ A onlyThrough a_exp (e_false) ->
-                                  M ⊢ A1 to A2 onlyThrough A3 ->
-                                  M ⊢ A1 ∧ A to A2 onlyThrough A3 ∧ A
+                                       M ⊢ A1 to A2 onlyThrough A3 ->
+                                       M ⊢ A1 ∧ A to A2 onlyThrough A3 ∧ A
 
   where
   "M '⊢' A1 'to' A2 'onlyThrough' A3" := (only_through M A1 A2 A3)
@@ -178,38 +180,47 @@ Module Inference(L : LanguageDef).
   | if1_classical : forall M P1 α C m β β' P2 P,
       M ⊢ {pre: ((a_class (e_addr α) C) ∧ P1 ∧ ¬ P) } (m_call α m β) {post: ¬ P2} ->
       β' = (fun v => Some (av_ v)) ∘ β  ->
-      M ⊢ (P1 ∧ (a_class (e_addr α) C) ∧ (∃x.[ (a♢ 0) calls (a_ α) ◌ (am_ m) ⟨ β' ⟩])) to1 P2 onlyIf P
+      M ⊢ (P1 ∧ (a_class (e_addr α) C) ∧ (∃x.[ (a♢ 0) calls (a_ α) ◌ m ⟨ β' ⟩])) to1 P2 onlyIf P
   | if1_wrapped : forall M α C P m β α',
       M ⊢ {pre: (a_class (e_addr α) C) ∧ ¬ P } (m_call α m β) {post: a_exp ((e♢ 0) ⩵̸ (e_ α'))} ->
-      M ⊢ (wrapped (a_ α') ∧ (a_class (e_ α) C) ∧ (∃x.[ (a♢ 0) calls (a_ α) ◌ (am_ m) ⟨ (fun v => Some (av_ v)) ∘ β ⟩ ]))
+      M ⊢ (wrapped (a_ α') ∧ (a_class (e_ α) C) ∧ (∃x.[ (a♢ 0) calls (a_ α) ◌ m ⟨ (fun v => Some (av_ v)) ∘ β ⟩ ]))
         to1 (¬ (wrapped (a_ α'))) onlyIf P
   | if1_internal : forall M A1 A2 A3,
       (forall C CDef m α β, ⟦ C ↦ CDef ⟧_∈ M ->
-                       m ∈ c_meths CDef ->
-      M ⊢ (A1 ∧ (a_class (e_ α) C) ∧ ∃x.[ (a♢ 0) calls (a_ α) ◌ (am_ m) ⟨ β ⟩]) to1 A2 onlyIf A3) ->
+                            m ∈ c_meths CDef ->
+                            M ⊢ (A1 ∧ (a_class (e_ α) C) ∧ ∃x.[ (a♢ 0) calls (a_ α) ◌ m ⟨ β ⟩]) to1 A2 onlyIf A3) ->
       M ⊢ A1 to1 A2 onlyIf A3
   | if1_if : forall M A1 A2 A3, M ⊢ A1 to A2 onlyIf A3 ->
                                 M ⊢ A1 to1 A2 onlyIf A3
   | if1_conseq : forall M A1 A1' A2 A2' A A', M ⊢ A1' to1 A2' onlyIf A' ->
-                                         M ⊢ A1 ⊇ A1' ->
-                                         M ⊢ A2 ⊇ A2' ->
-                                         M ⊢ A' ⊇ A ->
-                                         M ⊢ A1 to1 A2 onlyIf A
+                                              M ⊢ A1 ⊇ A1' ->
+                                              M ⊢ A2 ⊇ A2' ->
+                                              M ⊢ A' ⊇ A ->
+                                              M ⊢ A1 to1 A2 onlyIf A
   | if1_orI1  : forall M A1 A1' A2 A A', M ⊢ A1 to A2 onlyIf A ->
-                                    M ⊢ A1' to A2 onlyIf A' ->
-                                    M ⊢ A1 ∨ A1' to1 A2 onlyIf A ∨ A'
+                                         M ⊢ A1' to A2 onlyIf A' ->
+                                         M ⊢ A1 ∨ A1' to1 A2 onlyIf A ∨ A'
   | if1_orI2  : forall M A1 A2 A2' A A', M ⊢ A1 to1 A2 onlyIf A ->
-                                    M ⊢ A1 to1 A2' onlyIf A' ->
-                                    M ⊢ A1 to1 A2 ∨ A2' onlyIf A ∨ A'
+                                         M ⊢ A1 to1 A2' onlyIf A' ->
+                                         M ⊢ A1 to1 A2 ∨ A2' onlyIf A ∨ A'
   | if1_orE   : forall M A1 A2 A A', M ⊢ A1 to1 A2 onlyIf A ∨ A' ->
-                                M ⊢ A' to A2 onlyThrough a_exp (e_false) ->
-                                M ⊢ A1 to1 A2 onlyIf A
+                                     M ⊢ A' to A2 onlyThrough a_exp (e_false) ->
+                                     M ⊢ A1 to1 A2 onlyIf A
   | if1_andI : forall M A1 A2 A A', M ⊢ A1 to1 A2 onlyIf A ->
-                               M ⊢ A1 to1 A2 onlyIf A' ->
-                               M ⊢ A1 to1 A2 onlyIf A ∧ A'
+                                    M ⊢ A1 to1 A2 onlyIf A' ->
+                                    M ⊢ A1 to1 A2 onlyIf A ∧ A'
 
   where
   "M '⊢' A1 'to1' A2 'onlyIf' A3" := (only_if1 M A1 A2 A3).
+
+  Hint Constructors only_through only_if only_if1 : inference_db.
+
+
+  Scheme onlyThrough_mutind := Induction for only_through Sort Prop
+    with onlyIf_mutind := Induction for only_if Sort Prop
+    with onlyIf1_mutind := Induction for only_if1 Sort Prop.
+
+  Combined Scheme necessity_mutind from onlyThrough_mutind, onlyIf_mutind, onlyIf1_mutind.
 
   Close Scope inference_scope.
   Close Scope chainmail_scope.
